Quoting/unquoting of universes by S. Boulier
Add a command Make Definition := Eval ... in ...

add QuoteUniverses

theories/Ast.v
@@ -1,25 +1,13 @@
 Require Import Coq.Strings.String.
 Require Import Coq.PArith.BinPos.
 Require Import List. Import ListNotations.
-Require Import Template.monad_utils.
+From Template Require Import monad_utils.
+From Template Require Export univ uGraph.
 
 Definition ident := string. (* e.g. nat *)
 Definition kername := string. (* e.g. Coq.Init.Datatypes.nat *)
 
-
-Inductive level : Set :=
-| lProp
-| lSet
-| Level (_ : string)
-| LevelVar (_ : nat) (* these are debruijn indices *).
-
-Definition universe := list (level * bool). (* true if it is level+1 *)
-Definition uProp : universe := [(lProp, false)].
-Definition uSet : universe := [(lSet, false)].
-
-
-Inductive sort_family : Set :=
-| InProp | InSet | InType.
+Inductive sort_family : Set := InProp | InSet | InType.
 
 Inductive name : Set :=
 | nAnon
@@ -54,8 +42,6 @@ Record def (term : Set) : Set := mkdef
 Definition mfixpoint (term : Set) : Set :=
   list (def term).
 
-Definition universe_instance : Set := list level.
-
 Inductive term : Set :=
 | tRel       : nat -> term
 | tVar       : ident -> term (** For free variables (e.g. in a goal) *)
@@ -78,29 +64,20 @@ Inductive term : Set :=
 | tFix       : mfixpoint term -> nat -> term
 | tCoFix     : mfixpoint term -> nat -> term.
 
-Record inductive_body :=
-  mkinductive_body
-    { ind_name : ident;
-      ind_type : term; (* Closed arity *)
-      ind_kelim : list sort_family; (* Allowed elimination sorts *)
-      ind_ctors : list (ident * term (* Under context of arities of the mutual inductive *)
-                    * nat (* arity, w/o lets, w/o parameters *));
-      ind_projs : list (ident * term) (* names and types of projections, if any.
-                                     Type under context of params and inductive object *) }.
 
-Record minductive_decl :=
-  { ind_npars : nat;
-    ind_bodies : list inductive_body }.
+Definition mkApps t us :=
+  match us with
+  | nil => t
+  | _ => match t with
+        | tApp f args => tApp f (args ++ us)
+        | _ => tApp t us
+        end
+  end.
 
-Record constant_decl :=
-  { cst_universes : universe_instance;
-    cst_type : term;
-    cst_body : option term }.
+Definition mkApp t u := Eval cbn in mkApps t [u].
 
-Inductive global_decl :=
-| ConstantDecl : kername -> constant_decl -> global_decl
-| InductiveDecl : kername -> minductive_decl -> global_decl.
 
+(** * Entries *)
 
 (** representation of mutual inductives. nearly copied from Coq/kernel/entries.mli
 *)
@@ -132,48 +109,105 @@ Inductive recursivity_kind :=
   | BiFinite (** = non-recursive, like in "Record" definitions *).
 
 (* kernel/entries.mli*)
-Record definition_entry : Set := {
+Record definition_entry := {
   definition_entry_type : term;
-  definition_entry_body : term }.
-  (* Missing universes, opaque, inline *)
+  definition_entry_body : term;
+  definition_entry_polymorphic : bool;
+  definition_entry_universes   : universe_context;
+  definition_entry_opaque      : bool;
+ }.
+
 
 Record parameter_entry : Set := {
   parameter_entry_type : term }.
 
-Inductive constant_entry : Set :=
+Inductive constant_entry :=
 | ParameterEntry (p : parameter_entry)
 | DefinitionEntry (def : definition_entry).
 
-Record mutual_inductive_entry : Set := {
+Record mutual_inductive_entry := {
   mind_entry_record : option (option ident); 
   mind_entry_finite : recursivity_kind;
   mind_entry_params : list (ident * local_entry);
   mind_entry_inds : list one_inductive_entry;
   mind_entry_polymorphic : bool; 
-(*  mind_entry_universes : Univ.universe_context; *)
-  (* Should the above be used? At least we need one number indicating
-     the number of polymorphically bound definitions*)
+  mind_entry_universes : univ.universe_context;
   mind_entry_private : option bool
 }.
 
 
+(** * Declarations *)
 
-Inductive program : Set :=
-| PConstr : string -> universe_instance -> term (* type *) -> term (* body *) -> program -> program
-| PType   : ident -> nat (* # of parameters, w/o let-ins *) ->
+(** ** The context of De Bruijn indices *)
+
+Record context_decl := { decl_name : name ;
+                         decl_body : option term ;
+                         decl_type : term }.
+
+Definition vass x A := {| decl_name := x; decl_body := None; decl_type := A |}.
+Definition vdef x t A := {| decl_name := x; decl_body := Some t; decl_type := A |}.
+
+(* local ctx *)
+Definition context := list context_decl.
+
+Definition snoc {A} (Γ : list A) (d : A) := d :: Γ.
+
+Notation " Γ ,, d " := (snoc Γ d) (at level 20, d at next level).
+
+(** ** The context of global constants *)
+
+(* one_inductive_body from declarations.ml *)
+Record inductive_body :=
+  mkinductive_body
+    { ind_name : ident;
+      ind_type : term; (* Closed arity *)
+      ind_kelim : list sort_family; (* Allowed elimination sorts *)
+      ind_ctors : list (ident * term (* Under context of arities of the mutual inductive *)
+                    * nat (* arity, w/o lets, w/o parameters *));
+      ind_projs : list (ident * term) (* names and types of projections, if any.
+                                     Type under context of params and inductive object *) }.
+
+(* mutual_inductive_body from declarations.ml *)
+Record minductive_decl :=
+  { ind_npars : nat;
+    ind_bodies : list inductive_body ;
+    ind_universes : universe_context
+  }.
+
+(* constant_body from declarations.ml *)
+Record constant_decl :=
+  { cst_universes : universe_context;
+    cst_type : term;
+    cst_body : option term }.
+
+Inductive global_decl :=
+| ConstantDecl : kername -> constant_decl -> global_decl
+| InductiveDecl : kername -> minductive_decl -> global_decl.
+
+
+Definition global_declarations := list global_decl.
+
+Definition global_context : Type := global_declarations * uGraph.t.
+
+
+
+Inductive program :=
+| PConstr : string -> universe_context -> term (* type *) -> term (* body *) -> program -> program
+| PType   : ident -> universe_context -> nat (* # of parameters, w/o let-ins *) ->
             list inductive_body (* Non-empty *) -> program -> program
-| PAxiom  : ident -> universe_instance -> term (* the type *) -> program -> program
+| PAxiom  : ident -> universe_context -> term (* the type *) -> program -> program
 | PIn     : term -> program.
 
 Definition extend_program (p : program) (d : global_decl) : program :=
   match d with
   | ConstantDecl i {| cst_universes := u; cst_type:=ty;  cst_body:=Some body |}
-    => PConstr i u (* TODO universes *) ty body p
+    => PConstr i u ty body p
   | ConstantDecl i {| cst_universes := u; cst_type:=ty;  cst_body:=None |}
     => PAxiom i u ty p
-  | InductiveDecl i {| ind_npars:=n; ind_bodies := l |}
-    => PType i n l p
+  | InductiveDecl i {| ind_npars:=n; ind_bodies := l ; ind_universes := u |}
+    => PType i u n l p
   end.
+
 
 
 
@@ -219,6 +253,7 @@ Inductive TemplateMonad : Type -> Prop :=
 | tmQuoteRec : forall {A:Type}, A  -> TemplateMonad program
 (** Quote the body of a definition or inductive. Its name need not be fully qualified *)
 | tmQuoteInductive : kername -> TemplateMonad minductive_decl
+| tmQuoteUniverses : unit -> TemplateMonad uGraph.t
 | tmQuoteConstant : kername -> bool (** bypass opacity?*) -> TemplateMonad constant_entry
 | tmMkDefinition : ident -> term -> TemplateMonad unit
     (* unquote before making the definition *)
