test-suite/bugChecker.v
@@ -1,0 +1,26 @@
+(* -*- coq-prog-args : ("-debug" "-type-in-type") -*-  *)
+
+From Template Require Import Template Typing Checker Ast.
+Require Import List String. Import ListNotations.
+Set Printing Universes.
+
+Definition T := Type.
+Definition T' := T.
+Definition foo' := (T : T').
+
+Quote Recursively Definition p := foo'.
+Eval lazy in (let '(Σ, t) := decompose_program p ([], init_graph) in
+let t := (tSort (Universe.super (Level.Level "Top.10"))) in
+let u := (tSort (Universe.make (Level.Level "Top.10"))) in
+let Γ := [] in
+leq_term (snd Σ) t u).
+isconv (fst Σ) fuel (Cumul (snd Σ)) Γ t [] u []).
+
+
+    (*      convert_leq Σ [] (tSort (Universe.super (Level.Level "Top.10"))) *)
+    (*                  (tSort (Universe.make (Level.Level "Top.10")))). *)
+
+    (* infer Σ [] t). *)
+
+    (* let '(Σ, t) := decompose_program p ([], init_graph) in *)
+    (* check_wf_env Σ ;; infer_term Σ t. *)
