theories/LiftSubst.v
@@ -39,8 +39,8 @@ Fixpoint subst t k u :=
   | tRel n =>
     match nat_compare k n with
     | Datatypes.Eq => lift0 k t
-    | Gt => tRel n
-    | Lt => tRel (pred n)
+    | Datatypes.Gt => tRel n
+    | Datatypes.Lt => tRel (pred n)
     end
   | tEvar ev args => tEvar ev (List.map (subst t k) args)
   | tLambda na T M => tLambda na (subst t k T) (subst t (S k) M)
@@ -63,8 +63,12 @@ Fixpoint subst t k u :=
   | x => x
   end.
 
-Notation subst0 t u := (subst t 0 u).
+Notation subst0 t := (subst t 0).
 Notation "M { j := N }" := (subst N j M) (at level 10, right associativity).
+
+(** Substitutes [t1 ; .. ; tn] in u for [Rel 0; .. Rel (n-1)]*)
+Definition substl l t :=
+  List.fold_left (fun t u => subst0 u t) l t.
 
 Fixpoint closedn k (t : term) : bool :=
   match t with
