theories/TypingPlugin.v
@@ -2,10 +2,11 @@ From Template Require Import Ast Typing Checker.
 
 Require Import ExtrOcamlBasic.
 Require Import ExtrOcamlString.
+Require Import ExtrOcamlZInt.
 
 Set Extraction Optimize.
 
-Extraction Blacklist Ast String List Nat Typing.
+Extraction Blacklist uGraph univ Ast String List Nat Typing.
 
 Set Warnings "-extraction-opaque-accessed".
 
