theories/kernel/README.md
@@ -1,0 +1,1 @@
+The files of this directory are intented to follow the same scheme as those of the kernel directory of Coq's source code.
